@prefix rdf: <http://www.w3.org/1999/02/22-rdf-syntax-ns#> .
@prefix rdfs: <http://www.w3.org/2000/01/rdf-schema#> .
@prefix org: <http://www.w3.org/ns/org#> .
@prefix schema: <https://schema.org/> .
@prefix owl: <http://www.w3.org/2002/07/owl#> .
@prefix dcterms: <http://purl.org/dc/terms/> .
@prefix void: <http://rdfs.org/ns/void#> .
@prefix berorgs: <https://berlin.github.io/lod-vocabulary/berorgs/> .

# Vocabulary Terms

berorgs: a owl:Ontology ;
    rdfs:label "Berliner Organisationsvokabular"@de ;
    rdfs:label "Berlin Public Organisation Vocabulary"@en ;
    rdfs:comment """Ein Vokabular zur Beschreibung von Einheiten der Berliner Verwaltung. 
    Dies beinhaltet Typen von Organisationen, Arten von Unterorganisationen und Rollen, wie Abteilungen, und Beauftragte."""@de ;
    rdfs:comment """A vocabulary for describing organisations and organisational units of the Berlin public administration."""@en ;
    void:dataDump <https://raw.githubusercontent.com/berlin/lod-vocabulary/main/data/static/berorgs.ttl> ;
.

berorgs:Organogram a owl:Class ;
    rdfs:label "Organigramm"@de ;
    rdfs:label "organogram"@en ;
    rdfs:comment """Das Organisationsstruktur oder Organigramm einer Organisation,
    z.B. einer Behörde."""@de ;
    rdfs:comment """The organizational chart or organogram of an organization, e.g.
    a department within the public administration."""@en ;
    rdfs:isDefinedBy berorgs: ;
.

berorgs:contains a owl:ObjectProperty ;
    rdfs:label "enthält"@de ;
    rdfs:label "contains"@en;
    rdfs:comment """Diese Property bildet die Relation zwischen einem Organigramm und
    den in ihm enthaltenen Organisationen ab."""@de ;
    rdfs:comment """This property models the relation between an organogram and the
    organizations contained within it."""@en ;
    rdfs:domain berorgs:Organogram ;
    rdfs:range org:Organization ;
    rdfs:isDefinedBy berorgs: ;
.

# Organization Types

berorgs:Senatsverwaltung a owl:Class ;
    rdfs:label "Senate Department"@en ;
    rdfs:label "Senatsverwaltung"@de ;
    rdfs:comment """Senate Department, equivalent to ministries on a state level"""@en ;
    rdfs:comment """Senatsverwaltung, Ministerium des Landes Berlin"""@de ;
    rdfs:subClassOf schema:GovernmentOrganization ;
    rdfs:subClassOf schema:GovernmentOffice ;
    rdfs:subClassOf org:Organization ;
    rdfs:isDefinedBy berorgs: ;
.

berorgs:Senatskanzlei a owl:Class ;
    rdfs:label "Senate Chancellery"@en ;
    rdfs:label "Senatskanzlei"@de ;
    rdfs:comment """The Senate Chancellery represents the administrative office of the Senate in Berlin."""@en ;
    rdfs:comment """Die Senatskanzlei repräsentiert das Verwaltungsamt des Senats in Berlin."""@de ;
    rdfs:subClassOf schema:GovernmentOrganization ;
    rdfs:subClassOf schema:GovernmentOffice ;
    rdfs:subClassOf org:Organization ;
    rdfs:isDefinedBy berorgs: ;
    .

berorgs:OeffentlichesUnternehmen a owl:Class ; 
    rdfs:label "Public Enterprise"@en ;
    rdfs:label "Öffentliches Unternehmen"@de ;
    rdfs:comment """A public enterprise refers to an organization that is owned or controlled by the government and operates for the benefit of the public."""@en ;
    rdfs:comment """Ein öffentliches Unternehmen bezeichnet eine Organisation, die im Besitz oder unter Kontrolle der Regierung steht und zum Nutzen der Öffentlichkeit tätig ist."""@de ;
    rdfs:subClassOf schema:Organization ;
    rdfs:isDefinedBy berorgs: ;
    .

berorgs:Museum a owl:Class ; 
    rdfs:label "Museum"@en ;
    rdfs:label "Museum"@de ;
    rdfs:comment """Museum"""@en ;
    rdfs:comment """Museum"""@de ;
    rdfs:subClassOf schema:Museum ;
    rdfs:subClassOf schema:Organization ;
    rdfs:isDefinedBy berorgs: ;
.

berorgs:Amt a owl:Class ;
    rdfs:label "Office"@en ;
    rdfs:label "Amt"@de ;
    rdfs:comment """Describes a government agency tasked with a particular  on a state or municipal level."""@en ;
    rdfs:comment """Ein Amt beschreibt eine Behörde innerhalb einer Landes- oder Bezirksregierung."""@de ;
    rdfs:subClassOf schema:GovernmentOrganization ;
    rdfs:subClassOf schema:GovernmentOffice ;
    rdfs:subClassOf org:Organization ;
    rdfs:isDefinedBy berorgs: ;
.

berorgs:Bezirksamt a owl:Class ;
    rdfs:label "District Office"@en ;
    rdfs:label "Bezirksamt"@de ;
    rdfs:comment """The District Office represents the local administrative authority within a specific district."""@en ;
    rdfs:comment """Das Bezirksamt repräsentiert die örtliche Verwaltungsbehörde innerhalb eines bestimmten Bezirks."""@de ;
    rdfs:subClassOf berorgs:amt ;
    rdfs:subClassOf org:Organization ;
    rdfs:subClassOf schema:GovernmentOrganization ;
    rdfs:subClassOf schema:GovernmentOffice ; 
    rdfs:isDefinedBy berorgs: ;
.

berorgs:Landesamt a owl:Class ;
    rdfs:label "State Office"@en ;
    rdfs:label "Landesamt"@de ;
    rdfs:comment """The State Office represents a higher administrative authority at the state level."""@en ;
    rdfs:comment """Das Landesamt repräsentiert eine höhere Verwaltungsbehörde auf Landesebene."""@de ;
    rdfs:subClassOf berorgs:amt ;
    rdfs:subClassOf org:Organization ;
    rdfs:subClassOf schema:GovernmentOrganization ;
    rdfs:subClassOf schema:GovernmentOffice ; 
    rdfs:isDefinedBy berorgs: ;
.

berorgs:Landesstelle a owl:Class ;
    rdfs:label "Senate Department"@en ;
    rdfs:label "Landesstelle"@de ;
    rdfs:comment """A Landesstelle refers to a department or office within a state administration."""@en ;
    rdfs:comment """Landesstelle bezeichnet eine Abteilung oder Büro innerhalb einer Landesverwaltung."""@de ;
    rdfs:subClassOf schema:GovernmentOrganization ;
    rdfs:subClassOf schema:GovernmentOffice ; 
    rdfs:subClassOf org:Organization ; 
    rdfs:isDefinedBy berorgs: ;
.

berorgs:Leitstelle a owl:Class ;
    rdfs:label "Control Center"@en ;
    rdfs:label "Leitstelle"@de ;
    rdfs:comment """A Leitstelle is a central coordination and control center within the administration."""@en ;
    rdfs:comment """Eine Leitstelle ist ein zentrales Koordinations- und Kontrollzentrum innerhalb der Verwaltung."""@de ;
    rdfs:subClassOf schema:GovernmentOrganization ;
    rdfs:subClassOf schema:GovernmentOffice ; 
    rdfs:subClassOf org:Organization ; 
    rdfs:isDefinedBy berorgs: ;
.

berorgs:Fachbereich a owl:Class ;
    rdfs:label "Department Section"@en ;
    rdfs:label "Fachbereich"@de ;
    rdfs:comment """A Fachbereich represents a specialized department or area of expertise within the organization."""@en ;
    rdfs:comment """Ein Fachbereich repräsentiert eine spezialisierte Abteilung oder Fachgebiet innerhalb der Organisation."""@de ;
    rdfs:subClassOf org:Organization ;
    rdfs:isDefinedBy berorgs: ;
.

berorgs:Referat a owl:Class ;
    rdfs:label "Department"@en ;
    rdfs:label "Referat"@de ;
    rdfs:comment """A Referat is a specific section or division within a department, focusing on a particular subject."""@en ;
    rdfs:comment """Ein Referat ist eine spezifische Abteilung oder Sektion innerhalb eines Fachbereichs, die sich auf ein bestimmtes Thema konzentriert."""@de ;
    rdfs:subClassOf org:Organization ;
    rdfs:isDefinedBy berorgs: ;
.

berorgs:Abteilung a owl:Class ;
    rdfs:label "Division"@en ;
    rdfs:label "Abteilung"@de ;
    rdfs:comment """An Abteilung represents a larger administrative division or unit within the organization."""@en ;
    rdfs:comment """Eine Abteilung repräsentiert eine größere Verwaltungseinheit innerhalb der Organisation."""@de ;
    rdfs:subClassOf org:Organization ;
    rdfs:isDefinedBy berorgs: ;
.

berorgs:Serviceeinheit a owl:Class ;
    rdfs:label "Service Unit"@en ;
    rdfs:label "Serviceeinheit"@de ;
    rdfs:comment """A Service Unit is a unit within the organization dedicated to providing specific services."""@en ;
    rdfs:comment """Eine Serviceeinheit ist eine Einheit innerhalb der Organisation, die sich auf die Erbringung bestimmter Dienstleistungen spezialisiert hat."""@de ;
    rdfs:subClassOf org:Organization ;
    rdfs:isDefinedBy berorgs: ;
.

berorgs:Organisationseinheit a owl:Class ;
    rdfs:label "Organizational Unit"@en ;
    rdfs:label "Organisationseinheit"@de ;
    rdfs:comment """An Organizational Unit represents a general organizational unit within the structure of the entity."""@en ;
    rdfs:comment """Eine Organisationseinheit repräsentiert eine allgemeine organisatorische Einheit innerhalb der Struktur der Organisation."""@de ;
    rdfs:subClassOf org:Organization ;
    rdfs:isDefinedBy berorgs: ;
.

berorgs:NachgeordneteEinrichtung a owl:Class ;
    rdfs:label "Subordinate Institution"@en ;
    rdfs:label "Nachgeordnete Einrichtung"@de ;
    rdfs:comment """A Subordinate Institution refers to an institution or entity that is subordinate to the main organization."""@en ;
    rdfs:comment """Nachgeordnete Einrichtung bezeichnet eine Institution oder Einrichtung, die der Hauptorganisation untergeordnet ist."""@de ;
    rdfs:subClassOf org:Organization ;
    rdfs:isDefinedBy berorgs: ;
.

berorgs:Stabsstelle a owl:Class ;
    rdfs:label "Staff Unit"@en ;
    rdfs:label "Stabsstelle"@de ;
    rdfs:comment """A Stabsstelle refers to a specialized unit within the organization that provides support and advisory services to the management or leadership."""@en ;
    rdfs:comment """Eine Stabsstelle bezeichnet eine spezialisierte Einheit innerhalb der Organisation, die Unterstützungs- und Beratungsdienstleistungen für das Management oder die Führungsebene bereitstellt."""@de ;
    rdfs:subClassOf org:Organization ;
    rdfs:isDefinedBy berorgs: ;
.

berorgs:Leitungsstab a owl:Class ;
    rdfs:label "Management Staff"@en ;
    rdfs:label "Leitungsstab"@de ;
    rdfs:comment """A Leitungsstab represents a staff or team directly supporting the leadership or management of the organization."""@en ;
    rdfs:comment """Der Leitungsstab repräsentiert Mitarbeiter oder ein Team, das die Führung oder das Management der Organisation direkt unterstützt."""@de ;
    rdfs:subClassOf org:Organization ;
    rdfs:isDefinedBy berorgs: ;
.

berorgs:Buero a owl:Class ;
    rdfs:label "Office"@en ;
    rdfs:label "Büro"@de ;
    rdfs:comment """A Büro represents a functional office or workspace within the organization."""@en ;
    rdfs:comment """Ein Büro repräsentiert ein funktionales Büro oder Arbeitsbereich innerhalb der Organisation."""@de ;
    rdfs:subClassOf org:Organization ;
    rdfs:isDefinedBy berorgs: ;
.

berorgs:Ressort a owl:Class ;
    rdfs:label "Section"@en ;
    rdfs:label "Ressort"@de ;
    rdfs:comment """A Ressort refers to a specialized department or section within the organization."""@en ;
    rdfs:comment """Ein Ressort bezeichnet eine spezialisierte Abteilung oder Sektion innerhalb der Organisation."""@de ;
    rdfs:subClassOf org:Organization ;
    rdfs:isDefinedBy berorgs: ;
.

berorgs:Justitiariat a owl:Class ;
    rdfs:label "Legal Department"@en ;
    rdfs:label "Justitiariat"@de ;
    rdfs:comment """The Justitiariat represents the legal department within the organization, responsible for legal matters and advice."""@en ;
    rdfs:comment """Das Justitiariat repräsentiert die Rechtsabteilung innerhalb der Organisation, zuständig für rechtliche Angelegenheiten und Beratung."""@de ;
    rdfs:subClassOf org:Organization ;
    rdfs:isDefinedBy berorgs: ;
.

berorgs:Fachdienst a owl:Class ;
    rdfs:label "Specialized Service"@en ;
    rdfs:label "Fachdienst"@de ;
    rdfs:comment """A Fachdienst refers to a specialized service or unit within the organization."""@en ;
    rdfs:comment """Ein Fachdienst bezeichnet einen spezialisierten Dienst oder eine Einheit innerhalb der Organisation."""@de ;
    rdfs:subClassOf org:Organization ;
    rdfs:isDefinedBy berorgs: ;
.

berorgs:Geschaeftsbereich a owl:Class ;
    rdfs:label " "@en ;
    rdfs:label "Geschäftsbereich"@de ;
    rdfs:comment """ """@en ;
    rdfs:comment """ """@de ;
    rdfs:subClassOf org:Organization ;
    rdfs:isDefinedBy berorgs: ;
.

berorgs:Geschaeftsstelle a owl:Class ;
    rdfs:label " "@en ;
    rdfs:label "Geschäftsstelle"@de ;
    rdfs:comment """ """@en ;
    rdfs:comment """ """@de ;
    rdfs:subClassOf org:Organization ;
    rdfs:isDefinedBy berorgs: ;
.

berorgs:Sekretariat a owl:Class ;
    rdfs:label " "@en ;
    rdfs:label "Sekretariat"@de ;
    rdfs:comment """ """@en ;
    rdfs:comment """ """@de ;
    rdfs:subClassOf org:Organization ;
    rdfs:isDefinedBy berorgs: ;
.

berorgs:Landesbetrieb a owl:Class ;
    rdfs:label " "@en ;
    rdfs:label "Landesbetrieb"@de ;
    rdfs:comment """ """@en ;
    rdfs:comment """ """@de ;
    rdfs:subClassOf org:Organization ;
    rdfs:isDefinedBy berorgs: ;
.

berorgs:Landesinstitut a owl:Class ;
    rdfs:label " "@en ;
    rdfs:label "Landesinstitut"@de ;
    rdfs:comment """ """@en ;
    rdfs:comment """ """@de ;
    rdfs:subClassOf org:Organization ;
    rdfs:isDefinedBy berorgs: ;
.

berorgs:Landesarchiv a owl:Class ;
    rdfs:label " "@en ;
    rdfs:label "Landesarchiv"@de ;
    rdfs:comment """ """@en ;
    rdfs:comment """ """@de ;
    rdfs:subClassOf org:Organization ;
    rdfs:isDefinedBy berorgs: ;
.

berorgs:Landeszentrale a owl:Class ;
    rdfs:label " "@en ;
    rdfs:label "Landeszentrale"@de ;
    rdfs:comment """ """@en ;
    rdfs:comment """ """@de ;
    rdfs:subClassOf org:Organization ;
    rdfs:isDefinedBy berorgs: ;
.

berorgs:AnstaltDesOeffentlichenRechts a owl:Class ;
    rdfs:label " "@en ;
    rdfs:label "Anstalt des öffentlichen Rechts"@de ;
    rdfs:comment """ """@en ;
    rdfs:comment """ """@de ;
    rdfs:subClassOf org:Organization ;
    rdfs:isDefinedBy berorgs: ;
.

berorgs:Stiftung a owl:Class ;
    rdfs:label " "@en ;
    rdfs:label "Stiftung"@de ;
    rdfs:comment """ """@en ;
    rdfs:comment """ """@de ;
    rdfs:subClassOf org:Organization ;
    rdfs:isDefinedBy berorgs: ;
.

berorgs:Gericht a owl:Class ;
    rdfs:label " "@en ;
    rdfs:label "Gericht"@de ;
    rdfs:comment """ """@en ;
    rdfs:comment """ """@de ;
    rdfs:subClassOf org:Organization ;
    rdfs:isDefinedBy berorgs: ;
.

berorgs:BVVBuero a owl:Class ;
    rdfs:label " "@en ;
    rdfs:label "BVV-Büro"@de ;
    rdfs:comment """ """@en ;
    rdfs:comment """ """@de ;
    rdfs:subClassOf org:Organization ;
    rdfs:isDefinedBy berorgs: ;
.

berorgs:Pressestelle a owl:Class ;
    rdfs:label " "@en ;
    rdfs:label "Pressestelle"@de ;
    rdfs:comment """ """@en ;
    rdfs:comment """ """@de ;
    rdfs:subClassOf org:Organization ;
    rdfs:isDefinedBy berorgs: ;
.

berorgs:Rechtsamt a owl:Class ;
    rdfs:label " "@en ;
    rdfs:label "Rechtsamt"@de ;
    rdfs:comment """ """@en ;
    rdfs:comment """ """@de ;
    rdfs:subClassOf org:Organization ;
    rdfs:isDefinedBy berorgs: ;
.

berorgs:SozialraumorientiertePlanungskoordination a owl:Class ;
    rdfs:label " "@en ;
    rdfs:label "Sozialraumorientierte Planungskoordination"@de ;
    rdfs:comment """ """@en ;
    rdfs:comment """ """@de ;
    rdfs:subClassOf org:Organization ;
    rdfs:isDefinedBy berorgs: ;
.

# Roles

berorgs:SenatorIn a owl:Class ;
    rdfs:label "senator"@en ;
    rdfs:label "Senator:in"@de ;
    rdfs:comment """A Senator, head of the respective Senate Department. Equivalent to Minister on a State Level."""@en ;
    rdfs:comment """Senator:in der jeweiligen Senatsverwaltung."""@de ;
    rdfs:subClassOf org:Role ;
    org:headOf berorgs:senatsverwaltung ;
    rdfs:isDefinedBy berorgs: ;
.

berorgs:Abteilungsleitung a owl:Class ;
    rdfs:label "Division Head"@en ;
    rdfs:label "Abteilungsleitung"@de ;
    rdfs:comment """The Division Head represents the leader or head of a specific division within the organization."""@en ;
    rdfs:comment """Die Abteilungsleitung repräsentiert die Führung oder Leitung einer spezifischen Abteilung innerhalb der Organisation."""@de ;
    rdfs:subClassOf org:Role ;
    org:headOf berorgs:abteilung ;
    rdfs:isDefinedBy berorgs: ;
.

berorgs:Referatsleitung a owl:Class ;
    rdfs:label "Department Head"@en ;
    rdfs:label "Referatsleitung"@de ;
    rdfs:comment """The Department Head represents the leader or head of a specific department within the organization."""@en ;
    rdfs:comment """Die Referatsleitung repräsentiert die Führung oder Leitung einer spezifischen Abteilung innerhalb der Organisation."""@de ;
    rdfs:subClassOf org:Role ;
    org:headOf berorgs:referat ;
    rdfs:isDefinedBy berorgs: ;
.

berorgs:LeitungDesLeitungsstabs a owl:Class ;
    rdfs:label "Head of Management Staff"@en ;
    rdfs:label "Leitung des Leitungsstabs"@de ;
    rdfs:comment """The Head of Management Staff represents the leader of the staff or team directly supporting the leadership or management of the organization."""@en ;
    rdfs:comment """Die Leitung des Leitungsstabs repräsentiert die Führung des Personals oder Teams, das die Führung oder das Management der Organisation direkt unterstützt."""@de ;
    rdfs:subClassOf org:Role ;
    rdfs:isDefinedBy berorgs: ;
.

berorgs:PressesprecherIn a owl:Class ;
    rdfs:label "Press Spokesperson"@en ;
    rdfs:label "Pressesprecher:in"@de ;
    rdfs:comment """The Press Spokesperson represents the official spokesperson for the respective organization, responsible for communication with the media."""@en ;
    rdfs:comment """Pressesprecher:innen repräsentieren die offiziellen Sprecher:innen der jeweiligen Organisation, zuständig für die Kommunikation mit den Medien."""@de ;
    rdfs:subClassOf org:Role ;
    rdfs:isDefinedBy berorgs: ;
.

berorgs:DatenschutzbeauftragteR a owl:Class ;
    rdfs:label "Data Privacy Officer"@en ;
    rdfs:label "Behördliche Datenschutzbeauftragte:r"@de ;
    rdfs:comment """The Data Privacy Officer represents the individual responsible for ensuring compliance with data protection laws and policies within the organization."""@en ;
    rdfs:comment """Datenschutzbeauftragte repräsentieren die Personen, die für die Einhaltung der Datenschutzgesetze und -richtlinien innerhalb der Organisation verantwortlich sind."""@de ;
    rdfs:subClassOf org:Role ;
    rdfs:isDefinedBy berorgs: ;
.

berorgs:Bueroleitung a owl:Class ;
    rdfs:label "Chief of Staff"@en ;
    rdfs:label "Büroleitung"@de ;
    rdfs:comment """The Chief of Staff represents the leader or head of the office within the organization."""@en ;
    rdfs:comment """Die Büroleitung repräsentiert die Führung oder Leitung des Büros innerhalb der Organisation."""@de ;
    rdfs:subClassOf org:Role ;
    rdfs:isDefinedBy berorgs: ;
.

berorgs:StaatssekretaerIn a owl:Class ;
    rdfs:label "State Secretary"@en ;
    rdfs:label "Staatssekretär:in"@de ;
    rdfs:comment """A State Secretary represents a high-ranking official responsible for assisting the head of a government department or ministry."""@en ;
    rdfs:comment """Staatssekretär:innen repräsentieren hochrangige Beamt:innen, die für die Unterstützung der Leitung einer Regierungsabteilung oder eines Ministeriums verantwortlich sind."""@de ;
    rdfs:subClassOf org:Role ;
    rdfs:isDefinedBy berorgs: ;
.

berorgs:ReferentIn a owl:Class ;
    rdfs:label "Specialist"@en ;
    rdfs:label "Referent:in"@de ;
    rdfs:comment """A Referent represents a specialist or expert within the organization, typically providing advice or expertise in a specific area."""@en ;
    rdfs:comment """Referent:innen repräsentieren Spezialist:innen oder Expert:innen innerhalb der Organisation, die in der Regel Beratung oder Fachkenntnisse in einem bestimmten Bereich bieten."""@de ;
    rdfs:subClassOf org:Role ;
    rdfs:isDefinedBy berorgs: ;
.

berorgs:BezirksbuergermeisterIn a owl:Class ;
    rdfs:label "District Mayor"@en ;
    rdfs:label "Bezirksbürgermeister:in"@de ;
    rdfs:comment """Chairperson of the district office of a district."""@en ;
    rdfs:comment """Vorsitzende:r des Bezirksamtes eines Bezirks."""@de ;
    rdfs:subClassOf org:Role ;
    rdfs:isDefinedBy berorgs: ;
.

berorgs:Leitung a owl:Class ;
    rdfs:label " "@en ;
    rdfs:label "Leitung"@de ;
    rdfs:comment """ """@en ;
    rdfs:comment """ """@de ;
    rdfs:subClassOf org:Role ;
    rdfs:isDefinedBy berorgs: ;
.

berorgs:Bueroleitung a owl:Class ;
    rdfs:label " "@en ;
    rdfs:label "Büroleitung"@de ;
    rdfs:comment """ """@en ;
    rdfs:comment """ """@de ;
    rdfs:subClassOf org:Role ;
    rdfs:isDefinedBy berorgs: ;
.

berorgs:BehoerdlicheRBeauftragteR a owl:Class ;
    rdfs:label " "@en ;
    rdfs:label "Behördliche:r Beauftragte:r"@de ;
    rdfs:comment """ """@en ;
    rdfs:comment """ """@de ;
    rdfs:subClassOf org:Role ;
    rdfs:isDefinedBy berorgs: ;
.

berorgs:LandesbeauftragteR a owl:Class ;
    rdfs:label " "@en ;
    rdfs:label "Landesbeauftragte:r"@de ;
    rdfs:comment """ """@en ;
    rdfs:comment """ """@de ;
    rdfs:subClassOf org:Role ;
    rdfs:isDefinedBy berorgs: ;
.

berorgs:Personalrat a owl:Class ;
    rdfs:label " "@en ;
    rdfs:label "Personalrat"@de ;
    rdfs:comment """ """@en ;
    rdfs:comment """ """@de ;
    rdfs:subClassOf org:Role ;
    rdfs:isDefinedBy berorgs: ;
.

berorgs:Frauenvertretung a owl:Class ;
    rdfs:label " "@en ;
    rdfs:label "Frauenvertretung"@de ;
    rdfs:comment """ """@en ;
    rdfs:comment """ """@de ;
    rdfs:subClassOf org:Role ;
    rdfs:isDefinedBy berorgs: ;
.

berorgs:Schwerbehindertenvertretung a owl:Class ;
    rdfs:label " "@en ;
    rdfs:label "Schwerbehindertenvertretung"@de ;
    rdfs:comment """ """@en ;
    rdfs:comment """ """@de ;
    rdfs:subClassOf org:Role ;
    rdfs:isDefinedBy berorgs: ;
.

berorgs:Auszubildendenvertretung a owl:Class ;
    rdfs:label " "@en ;
    rdfs:label "Auszubildendenvertretung"@de ;
    rdfs:comment """ """@en ;
    rdfs:comment """ """@de ;
    rdfs:subClassOf org:Role ;
    rdfs:isDefinedBy berorgs: ;
.

berorgs:DirektorIn a owl:Class ;
    rdfs:label " "@en ;
    rdfs:label "Direktor:in"@de ;
    rdfs:comment """ """@en ;
    rdfs:comment """ """@de ;
    rdfs:subClassOf org:Role ;
    rdfs:isDefinedBy berorgs: ;
.

berorgs:PraesidentIn a owl:Class ;
    rdfs:label " "@en ;
    rdfs:label "Präsident:in"@de ;
    rdfs:comment """ """@en ;
    rdfs:comment """ """@de ;
    rdfs:subClassOf org:Role ;
    rdfs:isDefinedBy berorgs: ;
.

berorgs:Amtsleitung a owl:Class ;
    rdfs:label " "@en ;
    rdfs:label "Amtsleitung"@de ;
    rdfs:comment """ """@en ;
    rdfs:comment """ """@de ;
    rdfs:subClassOf org:Role ;
    rdfs:isDefinedBy berorgs: ;
.

berorgs:Geschaeftsleitung a owl:Class ;
    rdfs:label " "@en ;
    rdfs:label "Geschäftsleitung"@de ;
    rdfs:comment """ """@en ;
    rdfs:comment """ """@de ;
    rdfs:subClassOf org:Role ;
    rdfs:isDefinedBy berorgs: ;
.

berorgs:VorsteherIn a owl:Class ;
    rdfs:label " "@en ;
    rdfs:label "Vorsteher:in"@de ;
    rdfs:comment """ """@en ;
    rdfs:comment """ """@de ;
    rdfs:subClassOf org:Role ;
    rdfs:isDefinedBy berorgs: ;
.

berorgs:AmtsleiterIn a owl:Class ;
    rdfs:label " "@en ;
    rdfs:label "Amtsleiter:in"@de ;
    rdfs:comment """ """@en ;
    rdfs:comment """ """@de ;
    rdfs:subClassOf org:Role ;
    rdfs:isDefinedBy berorgs: ;
.

berorgs:NachhaltigkeitsbeauftragteR a owl:Class ;
    rdfs:label " "@en ;
    rdfs:label "Nachhaltigkeitsbeauftragte:r"@de ;
    rdfs:comment """ """@en ;
    rdfs:comment """ """@de ;
    rdfs:subClassOf org:Role ;
    rdfs:isDefinedBy berorgs: ;
.

berorgs:IntegrationsbeauftragteR a owl:Class ;
    rdfs:label " "@en ;
    rdfs:label "Integrationsbeauftragte:r"@de ;
    rdfs:comment """ """@en ;
    rdfs:comment """ """@de ;
    rdfs:subClassOf org:Role ;
    rdfs:isDefinedBy berorgs: ;
.

berorgs:EuropabeauftragteR a owl:Class ;
    rdfs:label " "@en ;
    rdfs:label "Europabeauftragte:r"@de ;
    rdfs:comment """ """@en ;
    rdfs:comment """ """@de ;
    rdfs:subClassOf org:Role ;
    rdfs:isDefinedBy berorgs: ;
.

berorgs:BeauftragteRFuerPartnerschaften a owl:Class ;
    rdfs:label " "@en ;
    rdfs:label "Beauftragte:r für Partnerschaften"@de ;
    rdfs:comment """ """@en ;
    rdfs:comment """ """@de ;
    rdfs:subClassOf org:Role ;
    rdfs:isDefinedBy berorgs: ;
.

berorgs:BeauftragteRFuerEUUndStaedtepartnerschaften a owl:Class ;
    rdfs:label " "@en ;
    rdfs:label "Beauftragte:r für EU- und Städtepartnerschaften"@de ;
    rdfs:comment """ """@en ;
    rdfs:comment """ """@de ;
    rdfs:subClassOf org:Role ;
    rdfs:isDefinedBy berorgs: ;
.

berorgs:GleichstellungsbeauftragteR a owl:Class ;
    rdfs:label " "@en ;
    rdfs:label "Gleichstellungsbeauftragte:r"@de ;
    rdfs:comment """ """@en ;
    rdfs:comment """ """@de ;
    rdfs:subClassOf org:Role ;
    rdfs:isDefinedBy berorgs: ;
.

berorgs:BezirksstadtraetIn a owl:Class ;
    rdfs:label " "@en ;
    rdfs:label "Bezirksstadträt:in"@de ;
    rdfs:comment """ """@en ;
    rdfs:comment """ """@de ;
    rdfs:subClassOf org:Role ;
    rdfs:isDefinedBy berorgs: ;
.